Splinter/Journal/AllocationJournal.i.dfy
@@ -1,0 +1,319 @@
+// Copyright 2018-2021 VMware, Inc., Microsoft Inc., Carnegie Mellon University, ETH Zurich, and University of Washington
+// SPDX-License-Identifier: BSD-2-Clause
+
+include "LikesJournal.i.dfy"
+include "MiniAllocator.i.dfy"
+include "../Likes.i.dfy"
+
+// A Journal that keeps an in-memory index that maps each in-use LSN to the Address that stores it.
+// The impl will keep such an index so that Discard can return freed Addresses without having to
+// fault in the freed section of the journal to learn the chain of addresses involved.
+module AllocationJournal {
+  import opened Options
+  import opened MsgHistoryMod
+  import opened LSNMod
+  import opened Sequences
+  import opened Maps
+  import LikesJournal
+  import GenericDisk
+  import Mathematics
+  import opened LikesMod
+  import opened MiniAllocatorMod
+
+  type Pointer = GenericDisk.Pointer
+  type Address = GenericDisk.Address
+  type AU = GenericDisk.AU
+
+  type DiskView = LikesJournal.DiskView
+  type TruncatedJournal = LikesJournal.TruncatedJournal
+
+  /***************************************************************************************
+  *                                    Labels and defs                                   *
+  ***************************************************************************************/
+
+  datatype TransitionLabel =
+      ReadForRecoveryLabel(messages: MsgHistory)
+    | FreezeForCommitLabel(frozenJournal: TruncatedJournal)
+    | QueryEndLsnLabel(endLsn: LSN)
+    | PutLabel(messages: MsgHistory)
+    | DiscardOldLabel(startLsn: LSN, requireEnd: LSN)
+    // Internal-x labels refine to no-ops at the abstract spec
+    | InternalLabel(allocs: seq<Address>)  // Local No-op label
+  {
+    predicate WF() {
+      && (FreezeForCommitLabel? ==> frozenJournal.Decodable())
+    }
+
+    function I(): LikesJournal.TransitionLabel {
+      match this {
+        case ReadForRecoveryLabel(messages) => LikesJournal.ReadForRecoveryLabel(messages)
+        case FreezeForCommitLabel(frozenJournal) => LikesJournal.FreezeForCommitLabel(frozenJournal)
+        case QueryEndLsnLabel(endLsn) => LikesJournal.QueryEndLsnLabel(endLsn)
+        case PutLabel(messages) => LikesJournal.PutLabel(messages)
+        case DiscardOldLabel(startLsn, requireEnd) => LikesJournal.DiscardOldLabel(startLsn, requireEnd)
+        case InternalLabel(allocs) => LikesJournal.InternalLabel(allocs)
+      }
+    }
+  }
+
+
+  
+  /***************************************************************************************
+  *                                    State Machine                                     *
+  ***************************************************************************************/
+
+  datatype Variables = Variables(
+    journal: LikesJournal.Variables,
+    lsnAUIndex: map<LSN, AU>, // lsnAUAddrIndex maps in-repr lsn's to their AU addr
+    first: AU, // AU of the first journal record, boundarylsn can be found in this AU
+    miniAllocator: MiniAllocator
+  )
+  {
+    predicate WF() {
+      && journal.WF()
+    }
+
+    // LikesJournal.lsnIndex(lsn).au == lsnAUAddrIndex(lsn)
+    // every page in this AU is not in freeset
+
+    // lsnIndex.Values (repr) 
+    // (expand au => each page addr) >= lsnIndex.Values
+
+    // expand AU to 1 for each page
+  }
+
+  // group a couple definitions together
+  predicate OnlyAdvanceLikesJournal(v: Variables, v': Variables, lbl: TransitionLabel, step: Step)
+  {
+    && (step.ReadForRecoveryStep? || step.FreezeForCommitStep? || step.ObserveFreshJournalStep? || step.PutStep?)
+    && LikesJournal.NextStep(v.journal, v'.journal, lbl.I(), step.I())
+    && v' == v.(
+      journal := v'.journal
+    )
+  }
+
+  // function DiscardOldAndGarbageCollect(tj: TruncatedJournal, newBdy: LSN, keep: set<AU>) : TruncatedJournal
+  //   requires tj.WF()
+  //   requires tj.diskView.boundaryLSN <= newBdy
+  // {
+  //   var newEntries := MapRestrict(tj.diskView.entries, keep); 
+  //   var newDiskView := LikesJournal.DiskView(newBdy, newEntries);
+  //   if tj.SeqEnd() == newBdy
+  //   then LikesJournal.TruncatedJournal(None, newDiskView)
+  //   else LikesJournal.TruncatedJournal(tj.freshestRec, newDiskView)
+  // }
+
+//   // Update lsnAUIndex with by discarding lsn's strictly smaller than bdy
+//   function {:opaque} lsnAUIndexDiscardUpTo(lsnAUIndex: map<LSN, Address>, bdy: LSN) : (out: map<LSN, Address>)
+//     ensures IsSubMap(out, lsnAUIndex)
+//     ensures forall k | k in out :: bdy <= k
+//     ensures forall k | k in lsnAUIndex &&  bdy <= k :: k in out
+//   {
+//     map x: LSN | x in lsnAUIndex && bdy <= x :: lsnAUIndex[x]
+//   }
+
+  predicate DiscardOld(v: Variables, v': Variables, lbl: TransitionLabel) 
+  {
+    // Enabling conditions
+    && lbl.DiscardOldLabel?
+    && LikesJournal.Next(v.journal,  v'.journal, lbl.I())
+
+    && v' == v.(
+      journal := v'.journal
+    )
+
+    // journal unobserve everything at once
+//     && v.journal.WF()
+//     && v.journal.truncatedJournal.diskView.Acyclic()
+//     && v.journal.SeqStart() <= lbl.startLsn <= v.journal.SeqEnd()
+//     && lbl.requireEnd == v.journal.SeqEnd()
+//     && v.journal.truncatedJournal.CanDiscardTo(lbl.startLsn)
+//     // Define v'
+//     // Addrs to delete from likes are pages that are between the old LSN and new LSN,
+//     // excluding the page containing the new LSN boundary
+//     && var lsnAUIndex' := lsnAUIndexDiscardUpTo(v.lsnAUIndex, lbl.startLsn);
+//     && var keepAddrs := lsnAUIndex'.Values;
+//     && var unrefAddrs := v.lsnAUIndex.Values - keepAddrs;
+
+//     && v' == v.(
+//       journal := LikesJournal.Variables(
+//         DiscardOldAndGarbageCollect(v.journal.truncatedJournal, lbl.startLsn, keepAddrs),
+//         if v.journal.unmarshalledTail.seqStart <= lbl.startLsn
+//         then v.journal.unmarshalledTail.DiscardOld(lbl.startLsn)
+//         else v.journal.unmarshalledTail
+//       ),
+//       lsnAUIndex := lsnAUIndex'
+//   )
+  }
+
+//   // Give SingletonIndex map comprehension a named trigger
+//   predicate InRange(start: LSN, end: LSN, lsn: LSN) {
+//     start <= lsn < end
+//   }
+
+// TODO(jonh): XXX remove opaque & ensures
+  function /*{:opaque}*/ SingletonIndex(start: LSN, end: LSN, value: AU) : (index: map<LSN, AU>)
+//    ensures start<end ==> start in index
+  {
+    // Redundant domain predicate to provide both a trigger and a finite-set heuristic.
+    map x: LSN | /*InRange(start, end, x) &&*/ start <= x < end :: value
+  }
+
+  // Update lsnAUIndex with additional lsn's from a new record
+  function lsnAUIndexAppendRecord(lsnAUIndex: map<LSN, AU>, msgs: MsgHistory, au: AU) : (out: map<LSN, AU>)
+    requires msgs.WF()
+    requires msgs.seqStart < msgs.seqEnd
+    ensures (forall x | msgs.seqStart <= x < msgs.seqEnd :: x !in lsnAUIndex) 
+            ==> out.Values == lsnAUIndex.Values + {au}
+  {
+    // msgs is complete map from seqStart to seqEnd 
+    // comprehension condition is redundant: Contains gives a trigger, <= < gives finite heuristic.
+    var update := SingletonIndex(msgs.seqStart, msgs.seqEnd, au);
+    var out := MapUnion(lsnAUIndex, update);
+    assert (forall x | msgs.seqStart <= x < msgs.seqEnd :: x !in lsnAUIndex) 
+            ==> out.Values == lsnAUIndex.Values + {au} by {
+      // TODO: this be broken in likesjournal too
+    }
+    out
+  }
+
+  predicate InternalJournalMarshal(v: Variables, v': Variables, lbl: TransitionLabel, step: Step)
+  {
+    // Enabling conditions
+    && step.InternalJournalMarshalStep?
+    // relying on this to restrict cache/diskview behavior, should not reach into lsnAddrIndex
+    && LikesJournal.NextStep(v.journal, v'.journal, lbl.I(), step.I()) 
+    // state transition
+    && v.miniAllocator.CanAllocate(step.addr)
+    && var discardmsgs := v.journal.journal.unmarshalledTail.DiscardRecent(step.cut);
+    && v' == v.(
+      journal := v'.journal,
+      lsnAUIndex := lsnAUIndexAppendRecord(v.lsnAUIndex, discardmsgs, step.addr.au),
+      miniAllocator := v.miniAllocator.AllocateAndObserve(step.addr)
+    )
+  }
+
+  predicate InternalNoOp(v: Variables, v': Variables, lbl: TransitionLabel)
+  {
+    && lbl.InternalLabel?
+    && lbl.allocs == []
+    && v.WF()
+    && v' == v
+  }
+ 
+  // build LSN index by walking every page
+  function BuildLsnAUIndexPageWalk(dv: DiskView, root: Pointer) : map<LSN, AU> 
+    requires dv.Decodable(root)
+    requires dv.Acyclic()
+    // requires root.Some? ==> dv.boundaryLSN < dv.entries[root.value].messageSeq.seqEnd
+    decreases dv.TheRankOf(root)
+  {
+    if root.None? then map[]
+    else 
+      var currMsgs := dv.entries[root.value].messageSeq;
+      var update := SingletonIndex(
+        Mathematics.max(dv.boundaryLSN, currMsgs.seqStart), currMsgs.seqEnd, root.value.au);
+      MapUnion(BuildLsnAUIndexPageWalk(dv, dv.entries[root.value].CroppedPrior(dv.boundaryLSN)), update)
+  }
+
+  // store first AU in superblock and invariant that explains this, invariant info
+  lemma TransitiveRanking(dv: DiskView, root: Address, later: Address, first: AU)
+    requires dv.Decodable(Some(later))
+    requires dv.Acyclic()
+    requires root.au != first
+    requires root.au == later.au
+    requires root.page <= later.page
+    ensures dv.Decodable(Some(root))
+    // should be less than <= bc it's enough to prove termination, cause later is already < caller's root
+    ensures dv.TheRankOf(Some(root)) <= dv.TheRankOf(Some(later))
+    decreases later.page
+  {
+    var prior := dv.entries[later].CroppedPrior(dv.boundaryLSN);
+    // TODO: prove this once we have invariants
+    assume false;
+    if prior != Some(root) {
+      TransitiveRanking(dv, root, prior.value, first);
+    }
+  }
+
+  // root should be the first page of an AU, last is the last lsn in that AU
+  // first is the AU of the first journal record
+  function BuildLsnAUIndexAUWalk(dv: DiskView, root: Address, last: LSN, first: AU) : map<LSN, AU>
+    requires dv.Decodable(Some(root))
+    requires dv.Acyclic()
+    requires root.au != first
+    requires root.page == 0
+    // requires dv.boundaryLSN < dv.entries[root].messageSeq.seqEnd
+    decreases dv.TheRankOf(Some(root))
+  {
+    // we jump to the first page of each AU and perform an AU walk skipping over pages in the middle 
+      var currMsgs := dv.entries[root].messageSeq;
+      var update := SingletonIndex(
+        Mathematics.max(dv.boundaryLSN, currMsgs.seqStart), last, root.au);
+
+      var prior := dv.entries[root].CroppedPrior(dv.boundaryLSN);
+      var priorResult := 
+        if prior.None? then map[] else
+          if prior.value.au == first then BuildLsnAUIndexPageWalk(dv, prior)
+          else (TransitiveRanking(dv, prior.value.FirstPage(), prior.value, first);
+            BuildLsnAUIndexAUWalk(dv, prior.value.FirstPage(), currMsgs.seqStart, first));
+
+      MapUnion(priorResult, update)
+  }
+
+  function BuildLsnAUIndex(tj: TruncatedJournal, first: AU) : map<LSN, AU> 
+    requires tj.Decodable()
+  {
+    if tj.freshestRec.None? then map[]
+    else
+      // if we are looking at address from the first AU, just walk the pages
+      if tj.freshestRec.value.au == first then BuildLsnAUIndexPageWalk(tj.diskView, tj.freshestRec)
+      else
+        var last := tj.diskView.entries[tj.freshestRec.value].messageSeq.seqEnd;
+        TransitiveRanking(tj.diskView, tj.freshestRec.value.FirstPage(), tj.freshestRec.value, first);
+        BuildLsnAUIndexAUWalk(tj.diskView, tj.freshestRec.value.FirstPage(), last, first)
+  }
+
+  predicate Init(v: Variables, journal: TruncatedJournal, first: AU)
+  {
+    && LikesJournal.Init(v.journal, journal) 
+    && v == Variables(v.journal, BuildLsnAUIndex(journal, first), first, MiniAllocator(map[]))
+  }
+
+  datatype Step =
+      ReadForRecoveryStep(depth: nat)
+    | FreezeForCommitStep(depth: nat)
+    | ObserveFreshJournalStep()
+    | PutStep()
+    | DiscardOldStep()
+    | InternalJournalMarshalStep(cut: LSN, addr: Address)
+    | InternalNoOpStep()
+  {
+    function I() : LikesJournal.Step
+    {
+      match this {
+        case ReadForRecoveryStep(depth) => LikesJournal.ReadForRecoveryStep(depth)
+        case FreezeForCommitStep(depth) => LikesJournal.FreezeForCommitStep(depth)
+        case ObserveFreshJournalStep() => LikesJournal.ObserveFreshJournalStep()
+        case PutStep() => LikesJournal.PutStep()
+        case DiscardOldStep() => LikesJournal.DiscardOldStep()
+        case InternalJournalMarshalStep(cut, addr) => LikesJournal.InternalJournalMarshalStep(cut, addr)
+        case InternalNoOpStep() => LikesJournal.InternalNoOpStep()
+      }
+    }
+  }
+
+  predicate NextStep(v: Variables, v': Variables, lbl: TransitionLabel, step: Step)
+  {
+    match step {
+      case DiscardOldStep() => DiscardOld(v, v', lbl)
+      case InternalJournalMarshalStep(_, _) => InternalJournalMarshal(v, v', lbl, step)
+      case InternalNoOpStep() => InternalNoOp(v, v', lbl)
+      case _ => OnlyAdvanceLikesJournal(v, v', lbl, step)
+    }
+  }
+
+  predicate Next(v: Variables, v': Variables, lbl: TransitionLabel) {
+    exists step: Step :: NextStep(v, v', lbl, step)
+  }
+} // end module LikesJournal
