Splinter/Journal/MiniAllocator.i.dfy
@@ -1,0 +1,139 @@
+// Copyright 2018-2021 VMware, Inc., Microsoft Inc., Carnegie Mellon University, ETH Zurich, and University of Washington
+// SPDX-License-Identifier: BSD-2-Clause
+
+include "../Disk/GenericDisk.i.dfy"
+include "../../lib/Base/Maps.i.dfy"
+
+module MiniAllocatorMod {
+  import opened GenericDisk
+  import opened Maps
+
+  datatype PageAllocator = PageAllocator(
+    observed: set<Address>, // pages reachable from superblock Repr
+    reserved: set<Address> // pages reachable from stack ref
+  ) {
+    predicate WF(au: AU) {
+      // && observed !! reserved // does not have to be disjoint, cow case
+      && |observed + reserved| <= PageCount()
+      && (forall addr | addr in observed + reserved :: addr.WF())
+      && (forall addr | addr in observed + reserved:: addr.au == au)
+    }
+
+    predicate FreeAddr(addrs: set<Address>) {
+      && (forall addr | addr in addrs :: addr.WF())
+      && addrs !! (observed + reserved)
+    }
+
+    // get a stack reference
+    function Reserve(addrs: set<Address>) : PageAllocator
+      requires FreeAddr(addrs)
+    {
+      PageAllocator(observed, reserved + addrs)
+    }
+
+    // done with / returns a stack reference 
+    function UnReserve(addrs: set<Address>) : PageAllocator
+      requires addrs <= reserved
+    {
+      PageAllocator(observed, reserved - addrs)
+    }
+
+    function Observe(addrs: set<Address>) : PageAllocator
+    {
+      PageAllocator(observed+addrs, reserved)
+    }
+
+    function Unobserve(addrs: set<Address>) : PageAllocator
+      requires addrs <= observed
+    {
+      PageAllocator(observed-addrs, reserved)
+    }
+
+    function UnobserveAll() : PageAllocator
+    {
+      Unobserve(observed)
+    }
+
+    function Free(addrs: set<Address>) : PageAllocator
+      requires addrs <= observed + reserved 
+    {
+      PageAllocator(observed-addrs, reserved-addrs)
+    }
+
+    predicate NoObservedPages() {
+      && observed == {}
+    }
+
+    predicate NoOutstandingRefs () { // is this a bad name?
+      && reserved == {}
+    }
+  }
+
+  // maybe we track a set of au
+
+  datatype MiniAllocator = MiniAllocator(allocs: map<AU, PageAllocator>) {
+    predicate WF() {
+      && forall au | au in allocs :: allocs[au].WF(au)
+    }
+
+    // mini allocator's job is to allocate freespace and manage reserved pages
+    // as long as there are no reserved pages, it can be safely removed from the mini allocator
+    predicate CanRemove(au: AU) {
+      && au in allocs
+      && allocs[au].NoOutstandingRefs() 
+    }
+
+    // predicate FreeOnRemove(au: AU) {
+    //   && alloc.observed == {}
+    // }
+
+    // a set of AUs that belongs to the frozen freeset
+    function NotObservedAUs() : set<AU>
+    {
+      set au | au in allocs && allocs[au].NoObservedPages() :: au
+    }
+
+    // b+tree wouldn't do this
+    // journal use it to unobserve discarded AUs at once
+    function UnobserveAUs(aus: set<AU>) : MiniAllocator
+      requires aus <= allocs.Keys
+    {
+      MiniAllocator(map au | au in allocs :: 
+        if au in aus then allocs[au].UnobserveAll() else allocs[au])
+    }
+
+    predicate CanAllocate(addr: Address)
+    {
+      && addr.au in allocs
+      && allocs[addr.au].FreeAddr({addr})
+    }
+
+    function AllocateAndObserve(addr: Address) : MiniAllocator
+      requires CanAllocate(addr)
+    {
+      var result := allocs[addr.au].Observe({addr});
+      MiniAllocator(allocs[addr.au := result])
+    }
+
+    // remove all unobserved AUs from the mini allocator
+    // function PruneUnObserved() : MiniAllocator
+    // {
+    //   MiniAllocator(MapRestrict(allocs, set au | au in allocs && !allocs[au].NoObservedPages()))
+    // }
+
+    // remove AUs from the mini allocator
+    function Prune(aus: set<AU>) : MiniAllocator
+      requires forall au | au in aus :: au in allocs && CanRemove(au)
+    {
+      MiniAllocator(MapRestrict(allocs, set au | au in allocs.Keys - aus))
+    }
+
+    // All AUs = freeset AUs !! RC AUs !! Unobserved MiniAllocator AUs
+  }
+}
+
+// frozen freeset = freeset + unobserved AUs 
+// Allocated Unobserved = not in freeset, reachable from a stack reference
+// Observed = reachable from superblock
+
+
